Experiments on array struct pointers

ulib/experimental/Steel.PCM.ArrayStruct.Pointer.fst
@@ -21,10 +21,62 @@ module Mem = Steel.PCM.Memory
 module SizeT = Steel.SizeT
 module Map = FStar.Map
 
+
+open FStar.FunctionalExtensionality
 module PCM = Steel.PCM
 module UPCM = Steel.PCM.Unitless
+module UPCMBase = Steel.PCM.Unitless.Base
 
-#set-options "--fuel 1 --ifuel 1"
+#set-options "--fuel 2 --ifuel 2"
+
+noeq type declared_array_struct : Type u#(a+1) = {
+  descriptor: AS.array_struct_descriptor u#a;
+  pcm: UPCM.unitless_pcm (AS.array_struct_type descriptor)
+}
+
+let declared_array_struct_type (a: declared_array_struct u#a) : Type u#a =
+  AS.array_struct_type a.descriptor
+
+let declared_array_struct_pcm
+  (a: declared_array_struct u#a)
+    : UPCM.unitless_pcm (declared_array_struct_type a) =
+  a.pcm
+
+
+let declare_base (a: Type u#a) (pcm: UPCM.unitless_pcm a) : declared_array_struct u#a = {
+  descriptor = AS.DBase a;
+  pcm = pcm
+}
+
+let declare_array (base: declared_array_struct u#a) (len: Steel.SizeT.t)
+    : declared_array_struct u#a
+  =
+  {
+    descriptor = AS.DArray (base.descriptor) len;
+    pcm = AS.pointwise_array_pcm (AS.array_struct_type base.descriptor) len base.pcm;
+  }
+
+let declare_struct
+  (base: (AS.field_id ^-> option (declared_array_struct u#a)))
+  (name: string)
+    : declared_array_struct u#a
+  =
+  let field_descriptors = on _ (fun f ->
+      match base f with
+      | None -> None
+      | Some b -> Some b.descriptor
+  ) in
+  let field_types = AS.struct_field_type field_descriptors in
+  let field_pcms : (field: AS.field_id -> (UPCM.unitless_pcm (field_types field))) = fun f ->
+    match base f with
+    | None -> UPCMBase.exclusive_unitless_pcm
+    | Some b -> b.pcm
+  in
+  AS.struct_field_type_unroll_lemma field_descriptors;
+  {
+    descriptor = AS.DStruct (field_descriptors);
+    pcm = AS.pointwise_struct_pcm field_types field_pcms;
+  }
 
 type path_item : Type u#0 =
   | PEnd
@@ -32,26 +84,6 @@ type path_item : Type u#0 =
   | PField: field: AS.field_id -> path_item
 
 let path : Type u#0 = list path_item
-
-let array_structs_context : Type u#(a+1) = Map.t string (AS.array_struct_descriptor u#a)
-
-let declared_array_struct
-  (c: array_structs_context u#a)
-  = s:string{Map.contains c s}
-
-let declared_array_struct_descriptor
-  (#c: array_structs_context u#a)
-  (a: declared_array_struct c)
-  : Tot (AS.array_struct_descriptor u#a)
-  =
-  Map.sel c a
-
-let declared_array_struct_type
-  (#c: array_structs_context u#a)
-  (a: declared_array_struct c)
-  : Tot Type
-  =
-  AS.array_struct_type (declared_array_struct_descriptor a)
 
 let rec valid_path
   (d: AS.array_struct_descriptor u#a)
@@ -63,25 +95,64 @@ let rec valid_path
   | AS.DArray sub_d len, (PIndex i)::sub_path ->
     SizeT.v i < SizeT.v len /\
     valid_path sub_d sub_path
-  | AS.DStruct fields, (PField field)::sub_path ->
-    valid_path (fields field) sub_path
+  | AS.DStruct fields, (PField field)::sub_path -> begin
+    match fields field with
+    | None -> False
+    | Some sub_descr ->
+      valid_path sub_descr sub_path
+    end
   | _ -> False
 
 let qualified
   (p: path)
-  (#c: array_structs_context u#a)
-  (a: declared_array_struct c)
+  (a: declared_array_struct u#a)
   : Tot prop
-  = valid_path (declared_array_struct_descriptor a) p
+  = valid_path a.descriptor p
+
+let rec sub_array_struct
+  (a: declared_array_struct u#a)
+  (p: path{p `qualified` a})
+  : declared_array_struct u#a
+  =
+  match a.descriptor, p with
+  | AS.DBase _, _ ->
+     a
+  | AS.DArray sub_d len, (PIndex i)::sub_path ->
+    let sub_pcm : UPCM.unitless_pcm (AS.array_struct_type sub_d) =
+      admit()
+    in
+    sub_array_struct ({ descriptor = sub_d; pcm = sub_pcm }) sub_path
+  | _ -> admit()
+
 
 noeq type array_struct_ref
-  (#c: array_structs_context u#a)
-  (a: declared_array_struct c)
-  (pcm: UPCM.unitless_pcm (declared_array_struct_type a))
+  (a: declared_array_struct u#a)
   : Type u#0
   = {
   mem_ref: Mem.ref
-    (option (declared_array_struct_type a))
-    (UPCM.to_full_pcm_with_unit pcm);
+    (option (AS.array_struct_type a.descriptor))
+    (UPCM.to_full_pcm_with_unit a.pcm);
   path: (path:path{path `qualified` a})
 }
+
+open Steel.PCM.Memory
+
+let pts_to_array_struct
+  (#a: declared_array_struct)
+  (r: array_struct_ref a)
+  (v : declared_array_struct_type a)
+  : slprop u#a
+  = pts_to r.mem_ref (Some v)
+
+assume val read_array_struct
+  (#a: declared_array_struct)
+  (r: array_struct_ref a)
+  (e: inames)
+  (v0: Ghost.erased (declared_array_struct_type a))
+  : action_except
+    (v:(declared_array_struct_type a){
+      UPCM.compatible (declared_array_struct_pcm a) v0 v
+    })
+    e
+    (pts_to_array_struct r v0)
+    (fun v -> pts_to_array_struct r v)
